Step 1: Build the Divided Difference Table
The divided differences are calculated as:

𝑓
[
𝑥
𝑖
,
𝑥
𝑖
+
1
]
=
𝑓
(
𝑥
𝑖
+
1
)
−
𝑓
(
𝑥
𝑖
)
𝑥
𝑖
+
1
−
𝑥
𝑖
f[x 
i
​
 ,x 
i+1
​
 ]= 
x 
i+1
​
 −x 
i
​
 
f(x 
i+1
​
 )−f(x 
i
​
 )
​
 
𝑓
[
𝑥
𝑖
,
𝑥
𝑖
+
1
,
𝑥
𝑖
+
2
]
=
𝑓
[
𝑥
𝑖
+
1
,
𝑥
𝑖
+
2
]
−
𝑓
[
𝑥
𝑖
,
𝑥
𝑖
+
1
]
𝑥
𝑖
+
2
−
𝑥
𝑖
f[x 
i
​
 ,x 
i+1
​
 ,x 
i+2
​
 ]= 
x 
i+2
​
 −x 
i
​
 
f[x 
i+1
​
 ,x 
i+2
​
 ]−f[x 
i
​
 ,x 
i+1
​
 ]
​
 
and so on.

Let's do it carefully:

First-order divided differences:

First-order differences
𝑓
[
𝑥
0
,
𝑥
1
]
=
138
−
43
4
−
2
=
95
2
=
47.5
f[x 
0
​
 ,x 
1
​
 ]= 
4−2
138−43
​
 = 
2
95
​
 =47.5
𝑓
[
𝑥
1
,
𝑥
2
]
=
778
−
138
7
−
4
=
640
3
≈
213.33
f[x 
1
​
 ,x 
2
​
 ]= 
7−4
778−138
​
 = 
3
640
​
 ≈213.33
𝑓
[
𝑥
2
,
𝑥
3
]
=
1515
−
778
8
−
7
=
737
1
=
737
f[x 
2
​
 ,x 
3
​
 ]= 
8−7
1515−778
​
 = 
1
737
​
 =737
Second-order divided differences:

Second-order differences
𝑓
[
𝑥
0
,
𝑥
1
,
𝑥
2
]
=
213.33
−
47.5
7
−
2
=
165.83
5
≈
33.166
f[x 
0
​
 ,x 
1
​
 ,x 
2
​
 ]= 
7−2
213.33−47.5
​
 = 
5
165.83
​
 ≈33.166
𝑓
[
𝑥
1
,
𝑥
2
,
𝑥
3
]
=
737
−
213.33
8
−
4
=
523.67
4
≈
130.917
f[x 
1
​
 ,x 
2
​
 ,x 
3
​
 ]= 
8−4
737−213.33
​
 = 
4
523.67
​
 ≈130.917
Third-order divided difference:

Third-order difference
𝑓
[
𝑥
0
,
𝑥
1
,
𝑥
2
,
𝑥
3
]
=
130.917
−
33.166
8
−
2
=
97.751
6
≈
16.2918
f[x 
0
​
 ,x 
1
​
 ,x 
2
​
 ,x 
3
​
 ]= 
8−2
130.917−33.166
​
 = 
6
97.751
​
 ≈16.2918
Step 2: Write Newton’s Divided Difference Polynomial
The general form:

𝑃
(
𝑥
)
=
𝑓
(
𝑥
0
)
+
(
𝑥
−
𝑥
0
)
𝑓
[
𝑥
0
,
𝑥
1
]
+
(
𝑥
−
𝑥
0
)
(
𝑥
−
𝑥
1
)
𝑓
[
𝑥
0
,
𝑥
1
,
𝑥
2
]
+
(
𝑥
−
𝑥
0
)
(
𝑥
−
𝑥
1
)
(
𝑥
−
𝑥
2
)
𝑓
[
𝑥
0
,
𝑥
1
,
𝑥
2
,
𝑥
3
]
P(x)=f(x 
0
​
 )+(x−x 
0
​
 )f[x 
0
​
 ,x 
1
​
 ]+(x−x 
0
​
 )(x−x 
1
​
 )f[x 
0
​
 ,x 
1
​
 ,x 
2
​
 ]+(x−x 
0
​
 )(x−x 
1
​
 )(x−x 
2
​
 )f[x 
0
​
 ,x 
1
​
 ,x 
2
​
 ,x 
3
​
 ]
Substitute all values:

𝑃
(
𝑥
)
=
43
+
(
𝑥
−
2
)
(
47.5
)
+
(
𝑥
−
2
)
(
𝑥
−
4
)
(
33.166
)
+
(
𝑥
−
2
)
(
𝑥
−
4
)
(
𝑥
−
7
)
(
16.2918
)
P(x)=43+(x−2)(47.5)+(x−2)(x−4)(33.166)+(x−2)(x−4)(x−7)(16.2918)
Step 3: Estimate f(6)
Substitute 
𝑥
=
6
x=6:

First term:

43
43
Second term:

(
6
−
2
)
(
47.5
)
=
(
4
)
(
47.5
)
=
190
(6−2)(47.5)=(4)(47.5)=190
Third term:

(
6
−
2
)
(
6
−
4
)
(
33.166
)
=
(
4
)
(
2
)
(
33.166
)
=
8
(
33.166
)
=
265.328
(6−2)(6−4)(33.166)=(4)(2)(33.166)=8(33.166)=265.328
Fourth term:

(
6
−
2
)
(
6
−
4
)
(
6
−
7
)
(
16.2918
)
=
(
4
)
(
2
)
(
−
1
)
(
16.2918
)
=
(
−
8
)
(
16.2918
)
=
−
130.3344
(6−2)(6−4)(6−7)(16.2918)=(4)(2)(−1)(16.2918)=(−8)(16.2918)=−130.3344
Now sum up:

𝑃
(
6
)
=
43
+
190
+
265.328
−
130.3344
P(6)=43+190+265.328−130.3344
=
(
43
+
190
)
+
(
265.328
−
130.3344
)
=(43+190)+(265.328−130.3344)
=
233
+
134.9936
=233+134.9936
=
367.9936
=367.9936
Thus,

𝑓
(
6
)
≈
368
 ms
f(6)≈368 ms
​
 
Final Answer:
✅ Estimated performance time for input size 
6
6 is approximately 368 milliseconds.

Quick Summary Table of Calculations:

Calculation	Result
𝑓
[
𝑥
0
,
𝑥
1
]
f[x 
0
​
 ,x 
1
​
 ]	47.5
𝑓
[
𝑥
1
,
𝑥
2
]
f[x 
1
​
 ,x 
2
​
 ]	213.33
𝑓
[
𝑥
2
,
𝑥
3
]
f[x 
2
​
 ,x 
3
​
 ]	737
𝑓
[
𝑥
0
,
𝑥
1
,
𝑥
2
]
f[x 
0
​
 ,x 
1
​
 ,x 
2
​
 ]	33.166
𝑓
[
𝑥
1
,
𝑥
2
,
𝑥
3
]
f[x 
1
​
 ,x 
2
​
 ,x 
3
​
 ]	130.917
𝑓
[
𝑥
0
,
𝑥
1
,
𝑥
2
,
𝑥
3
]
f[x 
0
​
 ,x 
1
​
 ,x 
2
​
 ,x 
3
​
 ]	16.2918
Final 
𝑃
(
6
)
P(6)	368 ms
Would you also like me to draw the full divided difference table neatly and show the polynomial expanded step-by-step? (It will look nice if you're writing this for an exam!)
Should I proceed? 🚀








